src/Iris/Std/GenSetsInstances.lean
@@ -1,0 +1,80 @@
+/-
+Copyright (c) 2026 Sergei Stepanenko. All rights reserved.
+Released under Apache 2.0 license as described in the file LICENSE.
+-/
+
+import Iris.Std.GenSets
+import Std.Data.ExtTreeSet
+import Iris.Std.CoPset
+
+/-! ## LawfulSet Instances -/
+
+namespace Iris.Std
+
+open Iris.Std.Set
+
+/-! ### ExtTreeSet Instance -/
+
+namespace ExtTreeSet
+
+variable {α : Type _} {cmp : α → α → Ordering} [Std.TransCmp cmp]
+
+instance : Union (Std.ExtTreeSet α cmp) where
+  union := Std.ExtTreeSet.union
+
+instance : Inter (Std.ExtTreeSet α cmp) where
+  inter := Std.ExtTreeSet.inter
+
+instance : SDiff (Std.ExtTreeSet α cmp) where
+  sdiff := Std.ExtTreeSet.diff
+
+instance : Set (Std.ExtTreeSet α cmp) α where
+
+theorem mem_singleton_extTreeSet [Std.LawfulEqCmp cmp] {x y : α} :
+    x ∈ ({y} : Std.ExtTreeSet α cmp) ↔ x = y := by
+  simp only [Std.ExtTreeSet.singleton_eq_insert, Std.ExtTreeSet.mem_insert,
+    Std.LawfulEqCmp.compare_eq_iff_eq, Std.ExtTreeSet.not_mem_empty, or_false]
+  apply Iff.intro <;> rintro ⟨⟩ <;> rfl
+
+instance [Std.LawfulEqCmp cmp] :
+    LawfulSet (Std.ExtTreeSet α cmp) α where
+  ext _ _ h := Std.ExtTreeSet.ext_mem h
+  mem_empty := Std.ExtTreeSet.not_mem_empty
+  mem_singleton := mem_singleton_extTreeSet
+  mem_union := Std.ExtTreeSet.mem_union_iff
+  mem_inter := Std.ExtTreeSet.mem_inter_iff
+  mem_diff := Std.ExtTreeSet.mem_diff_iff
+
+instance [Std.LawfulEqCmp cmp] : FiniteSet (Std.ExtTreeSet α cmp) α where
+  toList s := s.toList
+
+instance [Std.LawfulEqCmp cmp] : LawfulFiniteSet (Std.ExtTreeSet α cmp) α where
+  mem_toList := Std.ExtTreeSet.mem_toList
+  toList_nodup := by
+    intro m
+    have e := Std.ExtTreeSet.distinct_toList (t := m)
+    simp only [List.Nodup]
+    have heq : (fun x1 x2 => x1 ≠ x2) = (fun a b => ¬cmp a b = Ordering.eq) := by
+      ext x1 x2; simp
+    rw [heq]
+    apply e
+
+end ExtTreeSet
+
+/-! ### CoPset Instance -/
+
+namespace CoPset
+
+instance : Set CoPset Pos where
+
+instance : LawfulSet CoPset Pos where
+  ext _ _ h := CoPset.ext h
+  mem_empty := CoPset.mem_empty
+  mem_singleton := CoPset.in_singleton
+  mem_union := CoPset.in_union
+  mem_inter := CoPset.in_inter
+  mem_diff := CoPset.in_diff
+
+end CoPset
+
+end Iris.Std
